Write/prove correct remaining Letrec simplifications

compiler/backend/pure_letrecScript.sml
@@ -7,23 +7,15 @@ open pure_expTheory pure_miscTheory top_sortTheory;
 val _ = new_theory "pure_letrec";
 
 (*
-
   The motivation for these Letrec simplifications is that the parser
   will produce a giant Letrec holding all the top-level functions. It
   makes sense to split this up and clean it up as much as possible early.
+*)
 
-  Plan for the Letrec simplifications:
+(*******************)
 
-    1. make a pass that ensures, for every Letrec xs y, that
-       ALL_DISTINCT (MAP FST xs)
-
-    2. split every Letrec according to top_sort_any, i.e. each Letrec becomes
-       one or more nested Letrecs
-
-    3. clean up pass:
-        - remove any Letrec xs y that only bind variables that are not free in y
-        - change any Letrec [(v,x)] y into Let v x y, when v not free in x
-
+(*
+  1. a pass that ensures, for every Letrec xs y, that ALL_DISTINCT (MAP FST xs)
 *)
 
 Definition make_distinct_def:
@@ -45,6 +37,12 @@ Termination
   WF_REL_TAC ‘measure exp_size’ >> rw [] >>
   Induct_on `xs` >> rw[] >> gvs[exp_size_def]
 End
+
+
+(*
+  2. split every Letrec according to top_sort_any, i.e. each Letrec becomes
+     one or more nested Letrecs
+*)
 
 Definition make_Letrecs_def:
   make_Letrecs [] e = e ∧
@@ -69,6 +67,43 @@ Definition split_all_def:
 Termination
   WF_REL_TAC `measure exp_size` >> rw [] >>
   Induct_on `xs` >> rw[] >> gvs[exp_size_def]
+End
+
+
+(*
+  3. clean up pass:
+     - remove any Letrec xs y that only bind variables that are not free in y
+     - change any Letrec [(v,x)] y into Let v x y, when v not free in x
+*)
+
+Definition clean_all_def:
+  clean_all (Letrec xs y) = (
+    let y' = clean_all y in
+    if DISJOINT (set (MAP FST xs)) (freevars y) then y' else
+    case xs of
+      [(v,x)] => if v ∈ freevars x then Letrec xs y else Let v x y'
+    | _ => Letrec xs y'
+    ) ∧
+  clean_all (Lam n x) = Lam n (clean_all x) ∧
+  clean_all (Prim p xs) = Prim p (MAP clean_all xs) ∧
+  clean_all (App x y) = App (clean_all x) (clean_all y) ∧
+  clean_all res = res
+Termination
+  WF_REL_TAC `measure exp_size` >> rw [] >>
+  Induct_on `xs` >> rw[] >> gvs[exp_size_def]
+End
+
+
+(*
+    Putting it all together:
+*)
+
+Definition simplify_def:
+  simplify e =
+    let d = distinct e in
+    let s = split_all d in
+    let c = clean_all s in
+    c
 End
 
 val _ = export_theory();
